src/HOL/Word/Traditional_Syntax.thy
@@ -1,0 +1,18 @@
+(*  Author:     Jeremy Dawson, NICTA
+*)
+
+section \<open>Operation variants with traditional syntax\<close>
+
+theory Traditional_Syntax
+  imports Main
+begin
+
+class semiring_bit_syntax = semiring_bit_shifts +
+  fixes test_bit :: \<open>'a \<Rightarrow> nat \<Rightarrow> bool\<close>  (infixl "!!" 100)
+    and shiftl :: \<open>'a \<Rightarrow> nat \<Rightarrow> 'a\<close>  (infixl "<<" 55)
+    and shiftr :: \<open>'a \<Rightarrow> nat \<Rightarrow> 'a\<close>  (infixl ">>" 55)
+  assumes test_bit_eq_bit: \<open>test_bit = bit\<close>
+    and shiftl_eq_push_bit: \<open>a << n = push_bit n a\<close>
+    and shiftr_eq_drop_bit: \<open>a >> n = drop_bit n a\<close>
+
+end
